Refine abstract memory model
In order to prove certain "relational" properties comparing pairs of
programs, their states (in particular, their initial) states need to be
inspected, and the initial memories of two "similar" programs should
reflect similarities in interfaces and code distribution.

This small extension to the abstract memory model, carrying over easily
to the concrete model used by the compiler, should be able to establish
at least a significant part of this connection (as discussed with
Jérémy).

Common/Memory.v
@@ -13,6 +13,7 @@ Module Type AbstractComponentMemory.
   Parameter alloc : t -> nat -> t * Block.id.
   Parameter load : t -> Block.id -> Block.offset -> option value.
   Parameter store : t -> Block.id -> Block.offset -> value -> option t.
+  Parameter domm : t -> {fset Block.id}.
 
   Axiom load_prealloc:
     forall bufs b i,
@@ -45,6 +46,15 @@ Module Type AbstractComponentMemory.
       exists m',
         store m b i v' = Some m'.
 
+  Axiom domm_prealloc :
+    forall bufs m,
+      prealloc bufs = m ->
+      size (domm m) = size bufs.
+
+  Axiom domm_alloc :
+    forall m m' n b,
+      alloc m n = (m', b) ->
+      size (domm m') = size (domm m) + 1.
 End AbstractComponentMemory.
 
 Module ComponentMemory : AbstractComponentMemory.
@@ -101,6 +111,8 @@ Module ComponentMemory : AbstractComponentMemory.
       else None
     | None => None
     end.
+
+  Definition domm (m : t) := @domm nat_ordType block (content m).
 
   Lemma load_prealloc:
     forall bufs b i,
@@ -184,6 +196,17 @@ Module ComponentMemory : AbstractComponentMemory.
     - by move=> /IH [chunk' ->]; eauto.
   Qed.
 
+  Lemma domm_prealloc :
+    forall bufs m,
+      prealloc bufs = m ->
+      size (domm m) = size bufs.
+  Admitted.
+
+  Lemma domm_alloc :
+    forall m m' n b,
+      alloc m n = (m', b) ->
+      size (domm m') = size (domm m) + 1.
+  Admitted.
 End ComponentMemory.
 
 Module ComponentMemoryExtra.
